progress on soundness proof

mc_reify/reflexivity_tacs.v
@@ -7,6 +7,11 @@ Require Import MirrorCore.RTac.Core.
 (*Require Import MirrorCharge.RTac.ReifyLemma.*)
 Require Import mc_reify.update_tycon.
 Require Import mc_reify.set_reif.
+Require Import mc_reify.solve_exprD.
+Require Import ExtLib.Tactics.
+Require Import MirrorCore.Lambda.ExprDsimul.
+Import ExprDenote.
+
 
 Section tbled.
 
@@ -20,7 +25,18 @@ Instance SS : SubstI.Subst subst (expr typ func) :=
 Let RSym_sym := RSym_sym tbl.
 Existing Instance RSym_sym.
 
+Existing Instance SubstOk_ctx_subst.
+Existing Instance SubstUpdate_ctx_subst.
+Existing Instance SubstUpdateOk_ctx_subst.
+Existing Instance RType_typ.
+Existing Instance Typ2_tyArr.
+Existing Instance Expr_expr.
+Existing Instance MA.
+Existing Instance Expr_ok_fs.
+Instance MentionsAnyOk : MentionsAnyOk MA _ _.
+Admitted.
 
+Ltac solve_exprD := solve_exprD.solve_exprD tbl.
 
 Definition REFLEXIVITYTAC : rtac typ (expr typ func) :=
 fun tus tvs n m c s e => 
@@ -28,19 +44,57 @@ fun tus tvs n m c s e =>
 | (App (App (Inj (inr (Other (feq ty)))) l) r) =>
   match @exprUnify (ctx_subst c) typ func _ _ _ _ _ 3
                                  tus tvs 0 l r ty s with
-    | Some s => RTac.Core.Solved s 
+    | Some su => RTac.Core.Solved su 
     | None =>  RTac.Core.Fail
   end
 | _ => RTac.Core.Fail
 end.
+Opaque type_cast.
 
 Lemma REFLEXIVITYTAC_sound  :
 rtac_sound (Expr_expr := func_defs.Expr_expr_fs tbl) REFLEXIVITYTAC.
 unfold rtac_sound.
 intros.
- unfold rtac_spec.
-simpl in *.
-Admitted.
+unfold REFLEXIVITYTAC in H.
+do 7 (match type of H with
+          | match ?g with _ => _ end = _ => destruct g eqn:?;
+                      try solve [simpl in H; subst; 
+                      try apply rtac_spec_Fail]
+        end).
+pose proof (exprUnify_sound).
+specialize (H0 (ctx_subst ctx) typ func  _ _ _ _ _ _ _ _ 
+
+_ _ 3).
+subst.
+red in H0. red in H0.
+unfold rtac_spec. simpl. intros.
+apply H0 with (tv' := nil) in Heqo1; auto. clear H0.
+destruct Heqo1.
+
+split. auto.
+forward. simpl in *.
+unfold propD in H4. unfold exprD'_typ0 in H4. 
+simpl in H4.
+
+solve_exprD.
+unfold exprT_App. simpl.
+destruct (pctxD_substD H1 H3).
+destruct H6.
+edestruct H2; eauto. 
+destruct H10.
+destruct (substD_pctxD _ H0 H3 H10).
+destruct H12.
+forward. inv_some.
+split. admit. (*what is this*)
+intros. 
+eapply Pure_pctxD. apply H12.
+intros. simpl in *.
+specialize (H11 us0 vs0).
+cut (x0 us0 vs0). intros. specialize (H11 H14).
+destruct H11. specialize (H15 HList.Hnil).
+apply H15. 
+admit. 
+Admitted. (*Qed.*)
 
 Definition REFLEXIVITY := REFLEXIVITYTAC.
 
@@ -73,16 +127,48 @@ Definition REFLEXIVITY_DENOTE (rtype : typ) {H: @RelDec.RelDec (typD rtype) eq}
    fun tus tvs lus lvs c s e => (
 match e with
 | (App (App (Inj (inr (Other (feq _)))) l) r) =>
-  match reflect tbl nil nil l rtype, reflect tbl nil nil r rtype with
+  match func_defs.reflect tbl nil nil l rtype, func_defs.reflect tbl nil nil r rtype with
   | Some v1, Some v2 => if @RelDec.rel_dec _ eq H v1 v2 then Solved s else Fail
   | _, _ => Fail
   end
 | _ => Fail
 end).
 
+Lemma REFLEXIVITY_DENOTE_sound (rtype : typ) {H: @RelDec.RelDec (typD rtype) eq}
+{H0: RelDec.RelDec_Correct H}: 
+rtac_sound (REFLEXIVITY_DENOTE rtype tbl).
+unfold rtac_sound.
+intros.
+unfold REFLEXIVITY_DENOTE in H1.
+repeat (match type of H1 with
+          | match ?g with _ => _ end = _ => destruct g eqn:?;
+                      try solve [simpl in H; subst; 
+                      try apply rtac_spec_Fail]
+        end).
+subst. simpl. intros. 
+split.
+unfold func_defs.reflect, exprD in *. simpl in *.
+solve_exprD. 
+forward. split. admit. 
+intros. 
+unfold propD, exprD'_typ0 in *.  simpl in H4.
+solve_exprD.
+unfold exprT_App. simpl.
+eapply Pure_pctxD. eauto.
+intros.
+unfold func_defs.reflect, exprD in *. simpl in *.
+forward. inv_some.
+inversion H0. rewrite rel_dec_correct in Heqb.
+admit. (*exprD' with nil same as with any environment?*)
+Qed.
+
 Definition REFLEXIVITY_BOOL := REFLEXIVITY_DENOTE tybool.
 
+Definition REFLEXIVITY_BOOL_sound := REFLEXIVITY_DENOTE_sound tybool.
+
 Definition REFLEXIVITY_CEXPR := REFLEXIVITY_DENOTE tyc_expr.
+
+Definition REFLEXIVITY_CEXPR_sound := REFLEXIVITY_DENOTE_sound tyc_expr.
 
 Instance RelDec_op_ctypes_beq : @RelDec.RelDec (option Ctypes.type) eq :=
   Option.RelDec_eq_option RelDec_ctype_beq.
@@ -91,5 +177,8 @@ Instance RelDec_Correct_op_ctypes_beq : RelDec.RelDec_Correct RelDec_op_ctypes_b
   Option.RelDec_Correct_eq_option RelDec_Correct_ctype_beq.
 
 Definition REFLEXIVITY_OP_CTYPE := REFLEXIVITY_DENOTE (tyoption tyc_type).
+
+Definition REFLEXIVITY_OP_CTYPE_sound := REFLEXIVITY_DENOTE_sound (tyoption tyc_type).
+
 
 End tbled.
