mc_reify/symexe.v
@@ -169,7 +169,7 @@ Definition SYMEXE_STEP
            | Some ((t, v, r, gt) , st) =>  
              match st with 
                | Sskip => APPLY_SKIP 
-               | Ssequence s1 s2 => APPLY_SEQ s1 s2  
+               | Ssequence s1 s2 => APPLY_SEQ s1 s2 
                | Sset id exp => THEN (APPLY_SET' id exp t v r gt) 
                                      (TRY (FIRST [REFLEXIVITY_MSUBST tbl; 
                                                    (REFLEXIVITY_BOOL tbl);
